Ex 1.11: a function f in iteraive and recursive processes

In this exericse, we're asked to write to versions of the same function (iterative and recursive). The recursive is very easy as it's a direct translation of the math formula. In fact, u can just read it and figure out what the math is.
```
(define (f-rec n)
  (cond ((= n 0) 0)
        ((= n 1) 1)
        ((= n 2) 2)
        (else (+ (f-rec (- n 1)) (* 2 (f-rec (- n 2))) (* 3 (f-rec (- n 3)))))))
```

Coming up with the iterative version was trickier. First, I needed to workoutsome examples to see if I could observe any patterns

```
f(0) = 0
f(1) = 1
f(2) = 2
f(3) = 1.f(2) + 2.f(1) + 3.f(0) = 4
f(4) = 1.f(3) + 2.f(2) + 3.f(1) = 11
f(5) = 1.f(4) + 2.f(3) + 3.f(2) = 25
... etc
```
What we can see is: if we start with a function f(a, b, c) where a = 2, b = 1, c = 0 then we can see that at each step:

previous result -> a

a -> b

b -> c

And in iterative processes, computations need to be performed at each step and produce intermediate results (unlike deferring them in recursive versions). the key computation for us we can deduce from our first non-trivial case that is $ f(3) =  1 x a + 2 x b + 3 x c $. Now, this whole f(3) becomes the a of the next step and as above current a -> next b, current b -> next c

iterative process
```
(define (f n)
  (f-iter 2 1 0 n))

(define (f-iter a b c count)
  (if (= count 0) c
  (f-iter (+ a (* 2 b) (* 3 c)) a b (- count 1))))
```
